

Laborator 6/

TEMA:

23) $f(x) = \frac{e^x}{e-1}, 0 \leq x \leq 1$

i) Dacă $x < 0$ atunci: $F(x) = 0$

ii) Dacă $0 \leq x \leq 1$ atunci:

$$F(x) = \int_{-\infty}^x f(t) dt = \int_0^x \frac{e^t}{e-1} dt = \frac{e^x - 1}{e-1}$$

iii) Dacă $x > 1$ atunci:

$$F(x) = \int_0^1 \frac{e^t}{e-1} dt = 1$$

$$\text{Cum } i, ii, iii \Rightarrow F(x) = \begin{cases} 0, & x < 0 \\ \frac{e^x - 1}{e-1}, & x \in [0, 1] \\ 1, & x \geq 1 \end{cases}$$

Pt $x \in [0, 1]$:

$$F(x) = u \Leftrightarrow \frac{e^x - 1}{e-1} = u \Leftrightarrow e^x = u(e-1) + 1 (=)$$

$$\Rightarrow x = \ln[u(e-1) + 1] \Rightarrow X = \ln[u(e-1) + 1]$$

24) $f(x) = \begin{cases} \frac{x-2}{2}, & 2 \leq x \leq 3 \\ 2 - \frac{x}{3}, & 3 \leq x \leq 6 \end{cases}$

i) Dacă $x < 2$: $F(x) = 0$

ii) Dacă $x \in [2, 3]$:

$$F(x) = \int_2^x \frac{t-2}{2} dt = \int_2^x \left(\frac{t}{2} - 1\right) dt = \frac{(x-2)^2}{4}$$

iii) Dacă $x \in [3, 6]$:

$$F(x) = \int_2^3 \frac{t-2}{2} dt + \int_3^x \left(2 - \frac{t}{3}\right) dt = \frac{t^2}{4} \Big|_2^3 - t \Big|_2^3 + \int_3^x \frac{6-t}{3} dt =$$

$$= \frac{1}{4} + \int_3^x \left(1 - \frac{t}{3}\right) dt = \frac{-x^2}{12} + x - 2$$

iv) Nach $x \geq 6$:

$$F(x) = \int_2^3 \frac{t-2}{2} dt + \int_3^6 \frac{6-t}{6} dt + \int_6^x \frac{2-\frac{t}{3}}{2} dt =$$

$$= \frac{1}{4} + t \Big|_3^6 - \frac{t^2}{12} \Big|_3^6 + 0 = 1$$

Um i), ii), iii), iv) zu

$$\Rightarrow F(x) = \begin{cases} 0, & x < 2 \\ \left(\frac{x-2}{2}\right)^2, & 2 \leq x < 3 \\ -\frac{x^2}{12} + x - 2, & 3 \leq x < 6 \\ 1, & x \geq 6 \end{cases}$$

Pf $x \in (2, 3)$: $\Rightarrow [0, \frac{1}{4})$

$$F(x) = u \Leftrightarrow \frac{(x-2)^2}{4} = u \Leftrightarrow x^2 - 4x + 4(1-u) = 0 \Leftrightarrow$$

$$\Rightarrow x = 1 + \sqrt{u} \Rightarrow x = 1 + \sqrt{u}$$

Pf $x \in (3, 6)$: $\Rightarrow \frac{-1+6-2}{2} = \frac{3}{2} = \frac{3}{4}$

$$F(x) = u \Leftrightarrow -\frac{x^2}{12} + x - 2 = u \Leftrightarrow -\frac{x^2}{12} + x - (2+u) = 0 \Leftrightarrow$$

$$\Leftrightarrow x^2 - 12x + 12(2+u) = 0 \Leftrightarrow x = 6 + 2\sqrt{3(1-u)} \Rightarrow$$

$$\Rightarrow x = 6 + 2\sqrt{3(1-u)}, u \in \left[\frac{3}{4}, \frac{14}{4}\right)$$

Sum $1-u \sim \text{Unif}(0,1) \Rightarrow x = 6 + 2\sqrt{3u}$,

25) $f(x) = \begin{cases} e^{2x}, & x < 0 \\ e^{-2x}, & x \geq 0 \end{cases}$

i) Nach $x < 0$:

$$F(x) = \int_0^x e^{2t} dt = \frac{1}{2} e^{2t} \Big|_0^x = \frac{e^{2x} - 1}{2}$$

ii) Nach $x \geq 0$:

$$F(x) = \int_0^x e^{-2t} dt = -\frac{1}{2} e^{-2t} \Big|_0^x = \frac{1 - e^{-2x}}{2}$$

Dim 1, ii) \Rightarrow

$$F(x) = \begin{cases} \frac{e^{2x} - 1}{2}, & x < 0 \\ \frac{1 - e^{-2x}}{2}, & x \geq 0 \end{cases}$$

Pf $x < 0 \Rightarrow u \leq 0$

$$F(x) = u \Leftrightarrow \frac{e^{2x} - 1}{2} = u \Leftrightarrow 2x = \ln(2u + 1) \Rightarrow x = \frac{1}{2} \ln(2u + 1)$$

Pf $x \geq 0 \Rightarrow u \geq 0$

$$F(x) = u \Leftrightarrow \frac{1 - e^{-2x}}{2} = u \Leftrightarrow x = -\frac{1}{2} \ln(1 - 2u)$$